lib: fix up Levity dependency tracking
Uses proof body terms to disambiguate the names encoutered in
dependency extraction, rather than using (for example)
Thm.full_prop_of.

The result is that this catches a few more missing dependencies,
enough to correctly identify unused lemmas large sessions
like CRefine.

lib/AutoLevity_Base.thy
@@ -71,6 +71,41 @@ val attribs_of: Proof.context -> thm -> string list;
 val used_facts: Proof.context option -> thm -> (string * thm) list;
 val used_facts_attribs: Proof.context -> thm -> (string * string list) list;
 
+(*
+  Returns the proof body form of the prop proved by a theorem.
+
+  Unfortunately, proof bodies don't contain terms in the same form as what you'd get
+  from things like `Thm.full_prop_of`: the proof body terms have sort constraints
+  pulled out as separate assumptions, rather than as annotations on the types of
+  terms.
+
+  It's easier for our dependency-tracking purposes to treat this transformed
+  term as the 'canonical' form of a theorem, since it's always available as the
+  top-level prop of a theorem's proof body.
+*)
+val proof_body_prop_of: thm -> term;
+
+(*
+  Get every (named) term that was proved in the proof body of the given thm.
+
+  The returned terms are in proof body form.
+*)
+val used_named_props_of: thm -> (string * term) list;
+
+(*
+  Distinguish whether the thm name "foo_3" refers to foo(3) or foo_3 by comparing
+  against the given term. Assumes the term is in proof body form.
+
+  The provided context should match the context used to extract the (name, prop) pair
+  (that is, it should match the context used to extract the thm passed into
+  `proof_body_prop_of` or `used_named_props_of`).
+
+  Returns SOME ("foo", SOME 3) if the answer is 'it refers to foo(3)'.
+  Returns SOME ("foo_3", NONE) if the answer is 'it refers to foo_3'.
+  Returns NONE if the answer is 'it doesn't seem to refer to anything.'
+*)
+val disambiguate_indices: Proof.context -> string * term -> (string * int option) option;
+
 (* Install toplevel hook for tracking command positions. *)
 
 val setup_command_hook: {trace_apply : bool} -> theory -> theory;
@@ -150,14 +185,12 @@ in
   | _ => NONE
 end
 
+fun maybe_nth idx xs = idx |> try (curry List.nth xs)
 
 fun fact_from_derivation ctxt prop xnm =
 let
   val facts = Proof_Context.facts_of ctxt;
   (* TODO: Check that exported local fact is equivalent to external one *)
-
-  fun maybe_nth idx xs = idx |> try (curry List.nth xs)
-
   fun check_prop thm = Thm.full_prop_of thm = prop
 
   fun entry (name, idx) =
@@ -200,12 +233,12 @@ in
   if is_some local_result then local_result else global_result ()
 end
 
+fun thms_of (PBody {thms,...}) = thms
+
 (* We recursively descend into the proof body to find dependent facts.
    We skip over empty derivations or facts that we fail to find, but recurse
    into their dependents. This ensures that an attempt to re-build the proof dependencies
    graph will result in a connected graph. *)
-
-fun thms_of (PBody {thms,...}) = thms
 
 fun proof_body_deps
   (filter_name: string -> bool)
@@ -255,6 +288,125 @@ let
   val attribs_of = attribs_of ctxt;
 
 in map (apsnd attribs_of) fact_nms end
+
+local
+  fun app3 f g h x = (f x, g x, h x);
+
+  datatype ('a, 'b) Either =
+      Left of 'a
+    | Right of 'b;
+
+  local
+    fun partition_map_foldr f (x, (ls, rs)) =
+      case f x of
+        Left l => (l :: ls, rs)
+      | Right r => (ls, r :: rs);
+  in
+    fun partition_map f = List.foldr (partition_map_foldr f) ([], []);
+  end
+
+  (*
+    Extracts the bits we care about from a thm_node: the name, the prop,
+    and (the next steps of) the proof.
+  *)
+  val thm_node_dest =
+    app3
+      Proofterm.thm_node_name
+      Proofterm.thm_node_prop
+      (Proofterm.thm_node_body #> Future.join);
+
+  (*
+    Partitioning function for thm_node data. We want to insert any named props,
+    then recursively find the named props used by any unnamed intermediate/anonymous props.
+  *)
+  fun insert_or_descend (name, prop, proof) =
+    if name = "" then Right proof else Left (name, prop);
+
+  (*
+    Extracts the next layer of proof data from a proof step.
+  *)
+  val next_level = thms_of #> List.map (snd #> thm_node_dest);
+
+  (*
+    Secretly used as a set, using `()` as the values.
+  *)
+  structure NamePropTab = Table(
+    type key = string * term;
+    val ord = prod_ord fast_string_ord Term_Ord.fast_term_ord);
+
+  val insert_all = List.foldr (fn (k, tab) => NamePropTab.update (k, ()) tab)
+
+  (*
+    Proofterm.fold_body_thms unconditionally recursively descends into the proof body,
+    so instead of only getting the topmost named props we'd get _all_ of them. Here
+    we do a more controlled recursion.
+  *)
+  fun used_props_foldr (proof, named_props) =
+    let
+      val (to_insert, child_proofs) =
+        proof |> next_level |> partition_map insert_or_descend;
+      val thms = insert_all named_props to_insert;
+    in
+      List.foldr used_props_foldr thms child_proofs
+    end;
+
+  (*
+    Extracts the outermost proof step of a thm (which is just "the proof of the prop of the thm").
+  *)
+  val initial_proof =
+    Thm.proof_body_of
+      #> thms_of
+      #> List.hd
+      #> snd
+      #> Proofterm.thm_node_body
+      #> Future.join;
+
+in
+  fun used_named_props_of thm =
+    let val used_props = used_props_foldr (initial_proof thm, NamePropTab.empty);
+    in used_props |> NamePropTab.keys
+    end;
+end
+
+val proof_body_prop_of =
+  Thm.proof_body_of
+    #> thms_of
+    #> List.hd
+    #> snd
+    #> Proofterm.thm_node_prop
+
+local
+  fun thm_matches prop thm = proof_body_prop_of thm = prop
+
+  fun entry ctxt prop (name, idx) =
+    name
+      |> try (Proof_Context.get_thms ctxt)
+      |> Option.mapPartial (maybe_nth (idx - 1))
+      |> Option.mapPartial (Option.filter (thm_matches prop))
+      |> Option.map (K (name, SOME idx))
+
+  fun warn_if_ambiguous
+      name
+      (idx_result: (string * int option) option)
+      (non_idx_result: (string * int option) option) =
+    if is_some idx_result andalso is_some non_idx_result
+    then warning (
+      "Levity: found two possible results for name " ^ quote name ^ " with the same prop:\n" ^
+      (@{make_string} (the idx_result)) ^ ",\nand\n" ^
+      (@{make_string} (the non_idx_result)) ^ ".\nUsing the first one.")
+    else ()
+
+in
+  fun disambiguate_indices ctxt (name, prop) =
+    let
+      val entry = entry ctxt prop
+      val idx_result = (base_and_index name) |> Option.mapPartial entry
+      val non_idx_result = (name, 1) |> entry |> Option.map (apsnd (K NONE))
+      val _ = warn_if_ambiguous name idx_result non_idx_result
+    in
+      merge_options (idx_result, non_idx_result)
+    end
+end
 
 (* We identify "apply" applications by the document position of their corresponding method.
    We can only get a document position out of "real" methods, so internal methods
